\documentclass[a4paper]{article}
\usepackage[utf8]{inputenc}
\usepackage{amsmath}
\usepackage{amssymb}
\usepackage{amsthm}
\usepackage{amsfonts}
\usepackage{BOONDOX-cal}
\usepackage{quiver}
\usepackage[a4paper, margin=1in]{geometry}
\usepackage{tikz}
\usepackage{tikzscale}
\usepackage{subcaption}
\usepackage{wrapfig}
\usepackage{multicol}
\usepackage{parskip}
\usepackage{hyperref}
\usepackage{biblatex}

\newcommand{\ran}{\textrm{Range}\,}
\newcommand{\bbN}{\mathbb{N}}
\newcommand{\bbR}{\mathbb{R}}
\newcommand{\bbC}{\mathbb{C}}
\newcommand{\bbA}{\mathbb{A}}
\newcommand{\bbG}{\mathbb{G}}
\newcommand{\bbL}{\mathbb{L}}

\newcommand{\ob}{\text{ob}}
%\newcommand{\hom}{\text{Hom}}
\newcommand{\id}{\text{id}}

%\newcommand{\sA}{\boldsymbol{\mathcal{A}}}
%\newcommand{\sB}{\boldsymbol{\mathcal{B}}}
\newcommand{\sA}{\mathbcal{A}}
\newcommand{\sB}{\mathbcal{B}}
\newcommand{\sK}{\mathbcal{K}}

\newcommand{\T}{\mathcal{T}}
\newcommand{\bT}{\mathbcal{T}}
\newcommand{\mettop}{\mathbcal{MetTop}}

\theoremstyle{definition}
\newtheorem{definition}{Definition}[section]
\def\definitionautorefname{Definition}

\newtheorem{theorem}[definition]{Theorem}
\def\theoremautorefname{Theorem}
\newtheorem{proposition}[definition]{Proposition}
\def\propositionautorefname{Proposition}
\newtheorem{lemma}[definition]{Lemma}
\def\lemmaautorefname{Lemma}
\newtheorem{corollary}[definition]{Corollary}
\def\corollaryautorefname{Corollary}

\theoremstyle{remark}
\newtheorem*{remark}{Remark}
\def\remarkautorefname{Remark}

\theoremstyle{remark}
\newtheorem{example}[definition]{Example}
\def\exampleautorefname{Ex.}

\addbibresource{handout.bib}

\title{\vspace*{-5ex}DMD Error Representation}

\author{\vspace*{-15ex}April Herwig}
\date{25.08.2024}

\begin{document}

\maketitle

% --------------------------------------------------

Given

\begin{itemize}
    \item system $S : \Omega \to \Omega$
    \item quadrature scheme $\left\{ (w_i, x_i) \right\}_i$
    \item samples $\left\{ y_i \right\}_i$, $y_i = S(x_i)$
    \item family $\left\{ \psi_j \right\}_j$ spanning a Hilbert space $\mathcal{H}$
\end{itemize}

Construct the matrices

\begin{equation*}
    \Psi_X = \begin{matrix}
        \psi_1 (x_1) & \ldots & \psi_N (x_1) \\
        \vdots & & \vdots \\
        \psi_1 (x_M) & \ldots & \psi_N (x_M) \\
    \end{matrix}
    , \quad 
    \Psi_Y = \begin{matrix}
        \psi_1 (y_1) & \ldots & \psi_N (y_1) \\
        \vdots & & \vdots \\
        \psi_1 (y_M) & \ldots & \psi_N (y_M) \\
    \end{matrix}
    .
\end{equation*}

EDMD constructs the Galerkin matrices 

\begin{equation*}
    G = \Psi_X^* W \Psi_X, \quad A = \Psi_X^* W \Psi_Y, \quad L = \Psi_Y^* W \Psi_Y. 
\end{equation*}

We have 

\begin{itemize}
    \item $\lim_{M \to \infty} G_{j k} = \left\langle \psi_j, \psi_k \right\rangle =: \mathbb{G}_{j k}$,
    \item $\lim_{M \to \infty} A_{j k} = \left\langle \psi_j, \mathcal{K}\psi_k \right\rangle =: \mathbb{A}_{j k}$,
    \item $\lim_{M \to \infty} L_{j k} = \left\langle \mathcal{K}\psi_j, \mathcal{K}\psi_k \right\rangle =: \mathbb{L}_{j k}$.
\end{itemize}

Consider a candidate eigenpair $(\lambda, g),\ g = \sum_{j}^{\infty} a_j \psi_j$ for $\mathcal{K}$. 

\begin{align*}
    \left\Vert (\mathcal{K} - \lambda I) g \right\Vert_{\mathcal{H}}^2
    &= \left\langle (\sK - \lambda I) g, (\sK - \lambda I) g \right\rangle \\
    &= \left\langle \sK g, \sK g \right\rangle - \lambda \left\langle \sK g, g \right\rangle - \bar{\lambda} \left\langle g, \sK g \right\rangle + \vert \lambda \vert^2 \left\langle g, g \right\rangle \\
    &= a^* \left( \mathbb{L} - \lambda \mathbb{A}^* - \bar{\lambda} \mathbb{A} + \vert \lambda \vert^2 \mathbb{G} \right) a . 
\end{align*}

Now if we consider the "standard" EDMD residual

\begin{align*}
    \left\Vert (\bbG^{-1} \bbA - \lambda) g \right\Vert_{\mathcal{H}}^2
    &= \left\langle (\bbG^{-1} \bbA - \lambda)g, (\bbG^{-1} \bbA - \lambda)g \right\rangle \\
    &= \left\langle \bbG^{-1} \bbA g, \bbG^{-1} \bbA g \right\rangle - \lambda \left\langle \bbG^{-1} \bbA g, g \right\rangle - \bar{\lambda} \left\langle g, \bbG^{-1} \bbA g \right\rangle + \vert \lambda \vert^2 \left\langle g, g \right\rangle \\
    &= a^* (\bbA^* (\bbG \bbG^*)^{-1} \bbA - \lambda (\bbG^{-1} \bbA)^* - \bar{\lambda} \bbG^{-1} \bbA + \vert \lambda \vert^2 \bbG) a . 
\end{align*}

Let us assume that $\left\{ \psi_i \right\}_i$ is an orthonormal basis, so that $\bbG = I$. 

\begin{equation*}
    \left\Vert (\bbG^{-1} \bbA - \lambda) g \right\Vert_{\mathcal{H}}^2
    -
    \left\Vert (\mathcal{K} - \lambda I) g \right\Vert_{\mathcal{H}}^2
    =
    a^* (\bbA^* \bbA - \bbL) a. 
\end{equation*}

Now, viewing $\bbA$ as an "infinite matrix" on $l^2(\mathbb{N}_0)$

\begin{align*}
    \left( \bbA^* \bbA \right)_{i j} 
    &= \sum_l \bbA^*_{i l} \bbA_{l j} \\
    &= \sum_l \left\langle \sK \psi_i, \psi_l \right\rangle \, \left\langle \psi_l, \sK \psi_j \right\rangle \\
    &= \left\langle \sum_l \left\langle \sK \psi_i, \psi_l \right\rangle \psi_l, \sK \psi_j \right\rangle \\
    &= \left\langle \sK \psi_i, \sK \psi_j \right\rangle \\
    &= \bbL_{i j}
\end{align*}

This is good. If we however only have access to the first $N$ basis elements, that is, we have a finite matrix $\tilde{\bbA} = (\bbA_{i j})_{i,j = 1}^N$, then

\begin{align*}
    \left( \tilde{\bbA}^* \tilde{\bbA} \right)_{i j} 
    &= \sum_{l=1}^N \tilde{\bbA}^*_{i l} \tilde{\bbA}_{l j} \\
    &= \sum_{l=1}^N \left\langle \sK \psi_i, \psi_l \right\rangle \, \left\langle \psi_l, \sK \psi_j \right\rangle \\
    &= \left\langle \sK \psi_i, \sK \psi_j \right\rangle - \left\langle \sum_{l=N+1}^\infty \left\langle \sK \psi_i, \psi_l \right\rangle \psi_l, \sK \psi_j \right\rangle \\
    &= \bbL_{i j} - \left\langle P^\perp \sK \psi_i, \sK, \psi_j \right\rangle \\
\end{align*}

where $P$ is the orthogonal projection onto $\text{span} \left\{ \psi_1, \ldots, \psi_N \right\}$, $P^\perp = I - P$. 

% --------------------------------------------------

%\nocite{*}
%\printbibliography

\end{document}
